Prove upper bound on reachability calculation.

deps/poulet4/lib/P4automata/Reachability.v
@@ -79,7 +79,7 @@ Section ReachablePairs.
     match s with
     | inl s =>
       let st := P4A.t_states a s in
-      if t1.(st_buf_len) + steps == P4A.state_size st
+      if Compare_dec.le_gt_dec (size (P4A.interp a) s) (t1.(st_buf_len) + steps)
       then List.map (fun r => {| st_state := r; st_buf_len := 0 |}) (possible_next_states st)
       else [{| st_state := t1.(st_state); st_buf_len := t1.(st_buf_len) + steps |}]
     | inr b => [{| st_state := inr false; st_buf_len := 0 |}]
@@ -206,31 +206,381 @@ Section ReachablePairs.
     apply reachable_states_expansive.
   Qed.
 
-  Lemma reachable_states_bound:
-    forall fuel bound r,
-      (* FIXME: this bound is wrong... *)
-      bound = (length (enum S1)) * (length (enum S2)) ->
-      List.incl (reachable_states' fuel r) (reachable_states' bound r).
+  Definition chain (l: list state_pair) :=
+    forall l1 l2 p1 p2,
+      l = l1 ++ [p1; p2] ++ l2 ->
+      List.In p2 (reachable_pair_step p1).
+
+  Lemma chain_split_left:
+    forall l1 l2,
+      chain (l1 ++ l2) ->
+      chain l1.
+  Proof.
+    unfold chain.
+    intros.
+    apply (H0 l0 (l3 ++ l2)).
+    repeat rewrite List.app_assoc.
+    f_equal.
+    now repeat rewrite <- List.app_assoc.
+  Qed.
+
+  Lemma chain_trivial:
+    forall p, chain [p].
+  Proof.
+    unfold chain; intros.
+    apply (f_equal (@List.length state_pair)) in H0.
+    repeat rewrite List.app_length in H0.
+    simpl in H0.
+    lia.
+  Qed.
+
+  Lemma chain_cons (p p': state_pair) (l: list state_pair):
+    chain (l ++ [p]) ->
+    List.In p' (reachable_pair_step p) ->
+    chain (l ++ [p; p']).
+  Proof.
+    unfold chain in *; intros.
+    destruct l2.
+    - simpl in *.
+      apply (f_equal (@List.rev state_pair)) in H2.
+      repeat rewrite List.rev_app_distr in H2.
+      simpl in H2.
+      inversion H2.
+      now subst.
+    - apply (f_equal (@List.removelast state_pair)) in H2.
+      replace [p; p'] with ([p] ++ [p']) in H2 by easy.
+      rewrite List.app_assoc in H2.
+      rewrite List.removelast_last in H2.
+      rewrite List.app_assoc in H2.
+      rewrite List.removelast_app in H2 by easy.
+      apply (H0 l1 (List.removelast (s :: l2))).
+      rewrite <- List.app_assoc in H2.
+      exact H2.
+  Qed.
+
+  Lemma nodup_trivial {X: Type} (x: X):
+    List.NoDup [x].
+  Proof.
+    constructor.
+    - easy.
+    - constructor.
+  Qed.
+
+  Lemma nodup_split_left {X: Type} (l1 l2: list X):
+    List.NoDup (l1 ++ l2) ->
+    List.NoDup l1.
+  Proof.
+    revert l2; induction l1; intros.
+    - constructor.
+    - inversion_clear H0.
+      constructor.
+      + contradict H1.
+        apply List.in_app_iff.
+        now left.
+      + now eapply IHl1 with (l2 := l2).
+  Qed.
+
+  Lemma reachability_sound fuel p r:
+    List.In p (reachable_states' fuel r) ->
+    exists lpre lpost s,
+      List.In s r /\
+      s :: lpost = lpre ++ [p] /\
+      chain (s :: lpost) /\
+      List.NoDup (s :: lpost).
+  Proof.
+    revert p r; induction fuel; intros.
+    - simpl in H0.
+      exists nil, nil, p.
+      simpl; repeat split; auto.
+      + apply chain_trivial.
+      + apply nodup_trivial.
+    - simpl in H0.
+      unfold reachable_step in H0.
+      rewrite List.nodup_In, List.in_app_iff in H0.
+      destruct H0; [|now apply IHfuel].
+      rewrite <- List.flat_map_concat_map,
+              List.in_flat_map_Exists,
+              List.Exists_exists in H0.
+      destruct H0 as [p' [? ?]].
+      apply IHfuel in H0.
+      destruct H0 as [lpre' [lpost' [s [? [? [? ?]]]]]].
+      destruct (List.in_dec state_pair_eq_dec p ([s] ++ lpost')).
+      + apply List.in_split in i.
+        destruct i as [l1 [l2 ?]].
+        exists l1.
+        destruct l1.
+        * exists nil, s.
+          simpl in *.
+          repeat split; auto.
+          -- now inversion_clear H5.
+          -- apply chain_trivial.
+          -- apply nodup_trivial.
+        * simpl in *.
+          exists (l1 ++ [p]), s.
+          repeat split; auto.
+          -- now inversion_clear H5.
+          -- rewrite H5 in H3.
+             apply chain_split_left with (l2 := l2).
+             inversion_clear H5.
+             simpl.
+             now rewrite <- List.app_assoc.
+          -- rewrite H5 in H4.
+             inversion_clear H5.
+             eapply nodup_split_left with (l4 := l2).
+             now rewrite <- List.app_comm_cons, <- List.app_assoc.
+      + exists (lpre' ++ [p']), (lpost' ++ [p]), s.
+        repeat split; auto.
+        * rewrite List.app_comm_cons.
+          now f_equal.
+        * rewrite List.app_comm_cons, H2.
+          rewrite <- List.app_assoc.
+          apply chain_cons; auto.
+          now rewrite <- H2.
+        * rewrite List.app_comm_cons.
+          apply NoDup_app; auto.
+          -- apply nodup_trivial.
+          -- intros.
+             contradict n.
+             inversion_clear n; try contradiction.
+             now subst.
+          -- intros.
+             inversion_clear H5; try contradiction.
+             now subst.
+  Qed.
+
+  Lemma reachability_complete':
+    forall lpost lpre s p r,
+      List.In s r ->
+      s :: lpost = lpre ++ [p] ->
+      chain (s :: lpost) ->
+      List.In p (reachable_states' (length lpost) r).
+  Proof.
+    induction lpost using List.rev_ind; intros.
+    - simpl.
+      destruct lpre.
+      + simpl in H1.
+        inversion H1.
+        now subst.
+      + apply (f_equal (@List.length state_pair)) in H1.
+        rewrite List.app_length in H1.
+        simpl in H1.
+        lia.
+    - simpl.
+      induction lpre using List.rev_ind.
+      + simpl in H1.
+        inversion H1.
+        apply (f_equal (@List.rev state_pair)) in H5.
+        simpl in H5.
+        rewrite List.rev_unit in H5.
+        discriminate.
+      + rewrite List.app_length; simpl.
+        replace (length lpost + 1) with (Datatypes.S (length lpost)) by lia; simpl.
+        unfold reachable_step.
+        rewrite List.nodup_In.
+        rewrite List.in_app_iff.
+        left.
+        rewrite <- List.flat_map_concat_map.
+        rewrite List.in_flat_map_Exists.
+        rewrite List.Exists_exists.
+        simpl in H1.
+        exists x0.
+        split.
+        * eapply IHlpost with (s := s); auto.
+          -- rewrite <- List.removelast_last with (a := x) at 1.
+             rewrite <- List.removelast_last with (a := p).
+             rewrite <- List.app_comm_cons.
+             rewrite H1.
+             reflexivity.
+          -- unfold chain in *; intros.
+             apply H2 with (l1 := l1) (l2 := l2 ++ [x]).
+             rewrite List.app_comm_cons, H3.
+             now repeat rewrite <- List.app_assoc.
+        * rewrite H1 in H2.
+          rewrite <- List.app_assoc in H2.
+          simpl in H2.
+          unfold chain in H2.
+          apply H2 with (l1 := lpre) (l2 := nil).
+          reflexivity.
+  Qed.
+
+  Lemma reachability_complete:
+    forall lpost lpre s p r n,
+      List.In s r ->
+      s :: lpost = lpre ++ [p] ->
+      chain (s :: lpost) ->
+      length lpost <= n ->
+      List.In p (reachable_states' n r).
   Proof.
     intros.
-    destruct (Compare_dec.le_gt_dec fuel bound).
-    - now apply reachable_states_mono_fuel.
-    - (* Plan:
-         1. Show that p is reachable from r with fuel if and only if
-            there exists a non-empty list of states l such that
-            - l is a chain
-            - l[0] appears in r
-            - l[-1] = p
-            - l does not have any duplicates
-            - |l| <= fuel + 2
-         2. Show that if l and c are such that
-            - every element of l appears in c; and
-            - l does not have any duplicates
-            then |l| <= |c|
-         3. Conclude that if p is reachable from r in fuel steps, then
-            p is also reachable from r in as many steps as there are pairs.
-       *)
-  Admitted.
+    apply reachable_states_mono_fuel with (f1 := length lpost); auto.
+    now apply reachability_complete' with (s := s) (lpre := lpre).
+  Qed.
+
+  Definition valid_state_templates : list (state_template S) :=
+    [{| st_state := inr false; st_buf_len := 0 |};
+     {| st_state := inr true; st_buf_len := 0 |}] ++
+    List.flat_map (fun s =>
+      List.map (fun n => {| st_state := inl s; st_buf_len := n |})
+               (List.seq 0 (size (P4A.interp a) s))
+      ) (List.map inl (enum S1) ++ List.map inr (enum S2)).
+
+  Definition valid_state_template (t: state_template S) :=
+    match st_state t with
+    | inr _ => st_buf_len t = 0
+    | inl s => st_buf_len t < size (P4A.interp a) s
+    end.
+
+  Lemma valid_state_templates_accurate:
+    forall t,
+      valid_state_template t ->
+      List.In t valid_state_templates.
+  Proof.
+    unfold valid_state_template; intros.
+    destruct t.
+    simpl in *.
+    destruct st_state.
+    - right; right.
+      rewrite List.in_flat_map_Exists.
+      rewrite List.Exists_exists.
+      exists s.
+      split.
+      + rewrite List.in_app_iff.
+        destruct s; [left | right];
+        rewrite List.in_map_iff;
+        exists s;
+        split; auto;
+        apply elem_of_enum.
+      + rewrite List.in_map_iff.
+        exists st_buf_len.
+        split; auto.
+        apply List.in_seq.
+        lia.
+    - destruct b; [right; left | left].
+      all: now f_equal.
+  Qed.
+
+  Lemma valid_state_templates_closed:
+    forall t,
+      valid_state_template t ->
+      (forall t' n,
+        List.In t' (advance n t (st_state t)) ->
+        valid_state_template t').
+  Proof.
+    unfold valid_state_template; intros.
+    destruct (st_state t) eqn:?.
+    - simpl in H1.
+      destruct (Compare_dec.le_gt_dec _ _).
+      + rewrite List.in_map_iff in H1.
+        destruct H1 as [? [? ?]].
+        rewrite <- H1; simpl.
+        destruct x; auto.
+        apply a.
+      + destruct H1; try contradiction.
+        rewrite <- H1.
+        simpl.
+        rewrite Heqs.
+        unfold P4A.t_states in g.
+        simpl in H0.
+        simpl.
+        lia.
+   - destruct H1.
+     + now rewrite <- H1.
+     + contradiction.
+  Qed.
+
+  Definition valid_state_pair (p: state_pair) :=
+    valid_state_template (fst p) /\ valid_state_template (snd p).
+
+  Definition valid_state_pairs :=
+    List.list_prod valid_state_templates valid_state_templates.
+
+  Lemma valid_state_pairs_closed:
+    forall p,
+      valid_state_pair p ->
+      (forall p',
+        List.In p' (reachable_pair_step p) ->
+        valid_state_pair p').
+  Proof.
+    unfold valid_state_pair in *; intros.
+    unfold reachable_pair_step in H1.
+    unfold reachable_pair_step' in H1.
+    destruct p, p'.
+    unfold snd in H1.
+    apply List.in_prod_iff in H1.
+    destruct H1.
+    simpl in H0; destruct H0.
+    simpl; split.
+    - eapply valid_state_templates_closed with (t := s); auto.
+      exact H1.
+    - eapply valid_state_templates_closed with (t := s0); auto.
+      exact H2.
+  Qed.
+
+  Lemma valid_state_pairs_accurate:
+    forall p,
+      valid_state_pair p ->
+      List.In p valid_state_pairs.
+  Proof.
+    intros.
+    destruct p.
+    unfold valid_state_pairs.
+    apply List.in_prod_iff.
+    unfold valid_state_pair in H0.
+    simpl in H0.
+    split; now apply valid_state_templates_accurate.
+  Qed.
+
+  Lemma chain_preserve_valid:
+    forall l p,
+      valid_state_pair p ->
+      chain (p :: l) ->
+      forall p',
+        List.In p' l ->
+        valid_state_pair p'.
+  Proof.
+    induction l; intros.
+    - contradiction.
+    - assert (valid_state_pair a0).
+      + apply (valid_state_pairs_closed H0).
+        now apply H1 with (l1 := nil) (l2 := l).
+      + destruct H2.
+        * subst; auto.
+        * apply IHl with (p := a0); auto.
+          unfold chain in *.
+          intros.
+          eapply H1 with (l1 := p :: l1) (l2 := l2).
+          simpl.
+          now f_equal.
+  Qed.
+
+  Lemma reachable_states_bound:
+    forall fuel r,
+      (forall p, List.In p r -> valid_state_pair p) ->
+      List.incl (reachable_states' fuel r)
+                (reachable_states' (length valid_state_pairs) r).
+  Proof.
+    intros.
+    intros ? ?.
+    apply reachability_sound in H1.
+    destruct H1 as [lpre [lpost [s [? [? [? ?]]]]]].
+    eapply reachability_complete with (s := s).
+    - auto.
+    - exact H2.
+    - exact H3.
+    - apply List.NoDup_incl_length; [now inversion H4 |].
+      clear H2.
+      induction lpost using List.rev_ind; intros; try easy.
+      apply List.incl_app.
+      + apply IHlpost.
+        * now apply chain_split_left with (l2 := [x]).
+        * now eapply nodup_split_left with (l2 := [x]).
+      + unfold List.incl; intros.
+        destruct H2; [subst | easy].
+        apply valid_state_pairs_accurate.
+        apply chain_preserve_valid with (p := s) (l := lpost ++ [a1]); auto.
+        rewrite List.in_app_iff; right.
+        apply List.in_eq.
+  Qed.
 
   Definition reachable_states n s1 s2 : state_pairs :=
     let s := ({| st_state := inl (inl s1); st_buf_len := 0 |},
